src/tactics/FStar.Tactics.Basic.fsti
@@ -94,7 +94,7 @@ val lax_on                 : unit -> tac bool
 val tadmit_t               : term -> tac unit
 val inspect                : term -> tac term_view
 val pack                   : term_view -> tac term
-val pack_currified         : term_view -> tac term
+val pack_curried           : term_view -> tac term
 val join                   : unit -> tac unit
 val lget                   : typ -> string -> tac term
 val lset                   : typ -> string -> term -> tac unit
