ulib/FStar.Tactics.Builtins.fsti
@@ -333,8 +333,8 @@ val inspect : term -> Tac term_view
 val pack    : term_view -> Tac term
 
 (** Similar to [pack] above, but does not flatten arrows, it leaves
-    then in a currified form instead *)
-val pack_currified : term_view -> Tac term
+    then in a curried form instead *)
+val pack_curried : term_view -> Tac term
 
 (** Join the first two goals, which must be irrelevant, in a single
 one by finding a maximal prefix of their environment and reverting
